more on bounds

theories/L6_PCPS/bounds.v
@@ -2,702 +2,165 @@ Require Import Coq.NArith.BinNat Coq.Relations.Relations Coq.MSets.MSets Coq.MSe
         Coq.Lists.List Coq.omega.Omega Coq.Sets.Ensembles Coq.micromega.Lia.
 
 Require Import L6.cps L6.eval L6.Ensembles_util L6.List_util L6.tactics L6.set_util
-        L6.logical_relations L6.logical_relations_cc L6.algebra.
+        L6.logical_relations L6.logical_relations_cc L6.algebra L6.inline_letapp.
 Require Import micromega.Lia.
 
 Import ListNotations.
 
 Open Scope alg_scope. 
-Section Temp.
 
-    Context {steps: Type} {Hr : @resource_exp steps}.
-
-    Definition remove_steps_letapp cenv (P1 P2 P3 : PostT) :=
-    forall (x f z : positive) (t : fun_tag) (ys : list map_util.M.elt) (e1 : exp)
-           (rho1 : map_util.M.t val)
-           (xs : list var) (e_b1 : exp) (v1 : val) (e2 e2' e_b2: exp) (rho2 rho2' rhoc2  rhoc1 : M.t val) 
-           (fl : fundefs) (h : var) (vs : list val) (rhoc1' : map_util.M.t val) (c1 c1' c2 c2' : steps),
-      rho1 ! f = Some (Vfun rhoc1 fl h) ->
-      get_list ys rho1 = Some vs ->
-      find_def h fl = Some (t, xs, e_b1) ->
-      set_lists xs vs (def_funs fl fl rhoc1 rhoc1) = Some rhoc1' ->
-      bstep_fuel cenv rhoc1' e_b1 (Res v1) c1 ->
-
-      P1 (e_b1, rhoc1', c1) (e_b2, rhoc2, c2) (* when inlined body makes a tail call *) \/
-      P1 (e_b1, rhoc1', c1) (e_b2, rhoc2, c2 <+> one (Ehalt z)) (* when inlined body returns *) ->
-      P2 (e1, M.set x v1 rho1, c1') (e2', rho2', c2') ->
-      P3 (Eletapp x f t ys e1, rho1, c1 <+> c1' <+> one (Eletapp x f t ys e1))
-         (e2, rho2, c2 <+> c2').
-
-
-  Definition remove_steps_letapp_OOT cenv (P1 P2 : PostT) :=
-    forall (x f z: positive) (t : fun_tag) (ys : list map_util.M.elt) (e1 : exp) (rho1 : map_util.M.t val)
-           (xs : list var) (e_b1 : exp) (r : res) (e2 e_b2 : exp) (rho2 rhoc1 : M.t val) (rhoc2 : env) 
-           (fl : fundefs) (h : var) (vs : list val) (rhoc1' : map_util.M.t val) (c1 c2 : steps),
-      rho1 ! f = Some (Vfun rhoc1 fl h) ->
-      get_list ys rho1 = Some vs ->
-      find_def h fl = Some (t, xs, e_b1) ->
-      set_lists xs vs (def_funs fl fl rhoc1 rhoc1) = Some rhoc1' ->
-      bstep_fuel cenv rhoc1' e_b1 r c1 ->
-      
-      P1 (e_b1, rhoc1', c1) (e_b2, rhoc2, c2) \/
-      P1 (e_b1, rhoc1', c1) (e_b2, rhoc2, c2 <+> one (Ehalt z)) ->
-      P2 (Eletapp x f t ys e1, rho1, c1 <+> one (Eletapp x f t ys e1)) (e2, rho2, c2). 
-
-
-End Temp.
 
 Section Bounds.
   
+
+  (* ***** Fuel ***** *)
   
-  Program Instance resource_tup : @resource fin (nat * nat) :=
-    { zero := (0, 0)%type;
+  Program Instance fuel_res_pre : @resource fin nat :=
+    { zero := 0;
+      one_i fin := 1;
+      plus x y  := x + y; }.
+  Solve Obligations with (simpl; lia).
+
+
+  Program Instance fuel_res_ordered : @ordered fin nat fuel_res_pre :=
+    { lt := Peano.lt }.
+  Solve Obligations with (intro; intros; simpl; lia).
+  Solve Obligations with (simpl; lia).
+  Next Obligation.
+    destruct (lt_dec x y); auto. right. eexists (x - y). lia.
+  Qed.
+  
+  Program Instance fuel_res_ones : @resource_ones fin nat fuel_res_pre. 
+
+  Program Instance fuel_res_hom : @nat_hom fin nat fuel_res_pre :=
+    { to_nat y := y }.
+
+  Program Instance fuel_res_exp : @exp_resource nat :=
+    { HRes := fuel_res_pre }.
+  
+  Instance fuel_res : @fuel_resource nat.
+  Proof.
+    econstructor.
+    eapply fuel_res_ordered.
+    eapply fuel_res_ones.
+    eapply fuel_res_hom.
+  Defined.
+
+
+  (* ***** Trace ***** *)
+
+  
+  Program Instance trace_res_pre : @resource fin (nat * nat) :=
+    { zero := (0, 0);
       one_i fin :=
         match fin with
-        | Four => (1, 1)
-        | Six => (1, 1)
+        | Four => (0, 1)
+        | Six => (0, 1)
         | _ => (1, 0)
         end;
-      plus x y  :=
-        let '(x1, x2) := x in
-        let '(y1, y2) := y in
-        (x1 + y1, x2 + y2);
+      plus x y := (fst x + fst y, snd x + snd y) }.
+  Solve Obligations with (simpl; lia).
+  Solve Obligations with (split; congruence).
+  Next Obligation. simpl. f_equal; lia. Qed.
+  Next Obligation. simpl. f_equal; lia. Qed.
+  Next Obligation. simpl. f_equal; lia. Qed.  
+
+  Program Instance trace_res_exp : @exp_resource (nat * nat) :=
+    { HRes := trace_res_pre }.
+  
+  Instance trace_res : @trace_resource (nat * nat).
+  Proof.
+    econstructor. eapply trace_res_exp.
+  Defined.
+
+
+  Section Inline_bound. 
+
+    (* bound for inlining *)
+    Definition inline_bound (L G : nat) : PostT := 
+      fun '(e1, rho1, c1, (t1, tapp1)) '(e2, rho2, c2, (t2, tapp2)) =>
+        c1 <= c2 + 2 * G * tapp1 + 2 * L /\
+        tapp1 <= tapp2 + 2 * G * tapp2 + L /\
+        t2 + tapp2 = c2. 
+
+    Context (cenv : ctor_env).
+
+    Ltac unfold_all :=
+      try unfold zero in *;
+      try unfold one_ctx in *;
+      try unfold one in *;
+      try unfold one_i in *;
+      try unfold HRes in *;
+      try unfold HRexp_f in *; try unfold fuel_res in *; try unfold fuel_res_exp in *; try unfold fuel_res_pre in *;
+      try unfold HRexp_t in *; try unfold trace_res in *; try unfold trace_res_exp in *; try unfold trace_res_pre in *.
+
+    Instance inline_bound_compat L G (Hi : L <= G) (Hg : G > 0):
+      Post_properties cenv (inline_bound L G) (inline_bound L G) (inline_bound G G). 
+    Proof.
+      constructor; (try (intro; intros; intro; intros; destruct cout1; destruct cout2;
+                         unfold inline_bound in *; unfold_all; simpl; split; [| split ]; lia)).
+      - intro; intros. intro; intros. destruct cout1; destruct cout2. destruct cout1'; destruct cout2'.
+        unfold inline_bound in *; unfold_all; simpl. destructAll. split. lia. split; lia.
+
+      - intro; intros. intro; intros. 
+        unfold inline_bound in *; unfold_all; simpl.
+        assert (c = 0). eapply Nat.lt_1_r. eassumption. subst. lia.
+      - intro; intros. unfold post_base'. 
+        unfold inline_bound in *; unfold_all; simpl. lia.
+      - intro; intros; unfold inline_bound in *.
+        destruct x as [[[? ?] ?] [? ?]]; destruct y as [[[? ?] ?] [? ?]]. split; [| split ]; lia.
+    Qed. 
+    
+    Lemma inline_bound_post_Eapp_l i G v t l rho1 x rho2 :
+      post_Eapp_l (inline_bound i G) (inline_bound (S i) G) v t l rho1 x rho2.
+    Proof.
+      intro; intros. unfold inline_bound in *. unfold_all. simpl in *.
+      destruct cout1; destruct cout2. simpl in *. destructAll. 
+      split; [| split ]; lia.
+    Qed.
+
+    Lemma inline_bound_remove_steps_letapp_OOT i j G : 
+      remove_steps_letapp_OOT cenv (inline_bound j G) (inline_bound (S (i + j)) G).
+    Proof.
+      intro; intros. unfold inline_bound in *. unfold_all. simpl in *.
+      destruct cout1; destruct cout2. simpl in *.
+      split; [| split ]; lia.
+    Qed.
+
+    Lemma inline_bound_remove_steps_letapp i j G : 
+      remove_steps_letapp cenv (inline_bound i G) (inline_bound j G) (inline_bound (S (i + j)) G).
+    Proof.
+      intro; intros. unfold inline_bound in *. unfold_all; simpl in *.
+      destruct cout1; destruct cout2. destruct cout1'; destruct cout2'. simpl in *. lia. 
+    Qed.    
+
+
+    (* This allows us to prove divergence preservation *)  
+    Lemma inline_bound_post_upper_bound L G :
+      post_upper_bound (inline_bound L G).
+    Proof.
+      intro; intros. unfold inline_bound in *. unfold_all.
+      eexists (fun x => (1 + 2 * G + 2 * G * 2 * G) * x + 2 * L * 2 * G + 2 * L).
+      intros. 
+      destruct cout1 as [t1 tapp1]; destruct cout2 as [t2 tapp2].
+
+      destruct H. destruct H0.
+      assert (Hleq : tapp1 <= cin2 + 2 * G * cin2 + L) by lia. clear H0 H1.
       
-      lt_i fin x y :=
-        let '(x1, x2) := x in
-        let '(y1, y2) := y in
-        match fin with
-        | Four => x1 < y1 
-        | Six => x1 < y1
-        | _ => x1 < y1
-        end;
-
-      to_nat x := fst x;
+      assert (Hleq' : (1 + 2 * G + 2 * G * 2 * G) * cin1 + 2 * L * 2 * G + 2 * L <=
+                      (1 + 2 * G + 2 * G * 2 * G) * cin2 + 2 * L * 2 * G + 2 * L).
+      { eapply le_trans. eassumption. eapply le_trans.
+        eapply plus_le_compat_r. eapply plus_le_compat_l. eapply mult_le_compat_l. eassumption.
+        lia. } 
       
-    }.
-  Solve Obligations with (try (split; congruence)).
-  Solve Obligations with (simpl; f_equal; try lia).
-  Next Obligation. simpl; f_equal; try lia. Qed.
-  Next Obligation. simpl; f_equal; try lia. Qed.
-  Next Obligation. simpl; f_equal; try lia. Qed.
-  Next Obligation.  
-    intro; intros.
-    destruct x as [? ?]. destruct y as [? ?]. destruct z as [? ?].
-    destruct i; try (simpl in *; lia).
-  Qed.
-  Next Obligation. intro; intros. destruct x as [? ?]. intro. destruct i; simpl in *; lia. Qed.
-  Next Obligation. destruct i; simpl; try eapply Compare_dec.lt_dec. Qed.
-  Next Obligation. intros H. destruct i; simpl; lia. Qed.
-  Next Obligation. destruct i; simpl; lia. Qed.
-  Next Obligation. destruct i; simpl in *; lia. Qed.
-  Next Obligation. 
-    (* simpl in *. *)
-    (* edestruct (Compare_dec.le_dec n0 n3); edestruct (Compare_dec.le_dec n1 n4); *)
-    (*   edestruct (Compare_dec.le_dec n n2). *)
-    (* - right. eexists (n3 - n0, n4 - n1, n2 - n). simpl. f_equal; [ f_equal | ]; lia. *)
-    (* - left. exists Four. lia. *)
-    (* - left. exists Six. lia. *)
-    (* - left. exists Six. lia. *)
-    (* - left. exists One. lia. *)
-    (* - left. exists One. lia. *)
-    (* - left. exists One. lia. *)
-    (* - left. exists One. lia. *)
-  Admitted. 
-  Next Obligation.
-    destruct i; simpl;
-    
-      try (edestruct (Compare_dec.lt_dec n0 1); [ now eauto  | right; eexists (n0 -1, n1, n); simpl; f_equal; [ f_equal | ]; lia]);
-      try (edestruct (Compare_dec.lt_dec n1 1); [ now eauto  | right; eexists (n0, n1 -1, n); simpl; f_equal; [ f_equal | ]; lia]).
-    
-  Admitted.
-  Next Obligation.
-    destruct i; simpl; try f_equal; lia.
-  Qed. 
-  Next Obligation.
-    intros Heq. destruct i; simpl in *; try lia.
-    (* inv H; inv Heq; try lia. *)
-  Qed.
-  Next Obligation.
-    destruct i; simpl; reflexivity.
-  Qed.
+      assert (Hleq'' : cin1 <= cin2).
+      { eapply Nat.add_le_mono_r in Hleq'. eapply Nat.add_le_mono_r in Hleq'.
+        eapply NPeano.Nat.mul_le_mono_pos_l in Hleq'. eassumption. lia. }
 
-  Program Instance resource_tup_e : @resource_exp (nat * nat).
-
-  (* (possible) bound for inlining *)
-  Definition inline_bound (L G : nat) : relation (exp * env * (nat * nat)) := 
-    fun '(e1, rho1, (c1, c2)) '(e2, rho2, (c1', c2')) =>
-      c1 <= c1' + 2 * G * c2' + 2 * L /\
-      c2 <= c2' + 2 * G * c2' + 2 * L.
-
-  Context (cenv : ctor_env).
-
-
-  Close Scope alg_scope.
-  
-  Instance inline_bound_compat L G (Hi : L <= G) :
-    Post_properties cenv (inline_bound L G) (inline_bound L G) (inline_bound G G). 
-  Proof.
-    constructor; try (intro; intros; intro; intros; unfold inline_bound in *; lia);
-    try now (intro; intros; intro; intros; unfold inline_bound in *;
-         destruct c1 as [? ?]; destruct c2 as [? ?]; destructAll; simpl;
-         split; lia). 
-    - intro; intros; intro; intros; unfold inline_bound in *.
-      destruct c1 as [? ?]. destruct c2 as [? ?].
-      destruct c1' as [? ?]. destruct c2' as [? ?].
-      destructAll. simpl. split; lia.
-    - intro; intros; intro; intros; unfold inline_bound in *. 
-      destruct c as [? ?]. simpl in *. split; lia.      
-    - intro; intros; intro; intros; unfold inline_bound in *. 
-      destruct c as [? ?]. simpl in *. split; lia.      
-    - intro; intros; unfold inline_bound in *.
-      destruct x as [[? ?] [? ?]]; destruct y as [[? ?] [? ?]].
-      destructAll. split; lia.
-  Qed. 
+      eexists (cin2 - cin1). simpl. lia.
+    Qed.
 
   
-  Lemma cost_exp_size_exp e :
-    1 = cost e.
-  Proof.
-    destruct e; simpl; lia.
-  Qed.
-  
-
-  (* Lemma inline_bound_Hpost_zero i G f ft ys rho1 e2 rho2 (Hleq : 1 <= i): *)
-  (*   post_zero (Eapp f ft ys) rho1 e2 rho2 (inline_bound i G). *)
-  (* Proof. *)
-  (*   intro; intros; unfold inline_bound in *.  *)
-  (*   destruct c as [? ?]. *)
-  (*   simpl. unfold lt_e in H. simpl in H. split; try lia. *)
-  (* Qed. *)
-
-  
-  Lemma inline_bound_post_Eapp_l i G v t l rho1 x rho2 :
-    post_Eapp_l (inline_bound i G) (inline_bound (S i) G) v t l rho1 x rho2.
-  Proof.
-    intro; intros. unfold inline_bound in *.
-    destruct c1 as [? ?].
-    destruct c2 as [? ?]. simpl. split; lia.
-  Qed.
-  
-  Lemma inline_bound_remove_steps_letapp i j G : 
-    remove_steps_letapp cenv (inline_bound i G) (inline_bound j G) (inline_bound (S (i + j)) G).
-  Proof.
-    intro; intros. unfold inline_bound in *.
-    destruct c1 as [? ?].
-    destruct c2 as [? ?].
-    destruct c1' as [? ?].
-    destruct c2' as [? ?].
-    simpl. inv H4. lia. simpl in *.
-    rewrite !NPeano.Nat.mul_add_distr_l, !Nat.mul_0_r in *. simpl in *.
-    lia. 
-  Qed.    
-
-  Lemma inline_bound_remove_steps_letapp_OOT i j G : 
-    remove_steps_letapp_OOT cenv (inline_bound j G) (inline_bound (S (i + j)) G).
-  Proof.
-    intro; intros. unfold inline_bound in *.
-    destruct c1 as [? ?].
-    destruct c2 as [? ?].
-    simpl. inv H4. lia. simpl in *.
-    rewrite !NPeano.Nat.mul_add_distr_l, !Nat.mul_0_r in *. simpl in *. lia.
-  Qed.
-      
-
-    
-    post_constr_compat'; post_proj_compat' .
-
-      11:{ intro; intros. unfold inline_bound in *.
-         destruct x as [[? ? ] ?]. destruct y as [[? ? ] ?]. eapply le_trans. eassumption.
-         eapply plus_le_compat_r. eapply mult_le_compat_l. eapply plus_le_compat_l.
-         eapply mult_le_compat_r. eassumption. }
-    
-    - (* constr *) intro; intros. intro; intros.
-      unfold inline_bound in *.
-      eapply le_trans. eapply plus_le_compat_r. eassumption.
-      assert (Hleq : cost_exp_env G e1 (map_util.M.set x (Vconstr t vs) rho1) <= cost_exp_env G (Econstr x t ys e1) rho1).
-      { unfold cost_exp_env. eapply Max.max_lub.
-        -- eapply le_trans; [| eapply Max.le_max_l ]. simpl. lia.
-        -- eapply le_trans. eapply max_env_set.
-           eapply Max.max_lub; [| lia ]. eapply le_trans.
-           simpl. eapply max_env_getlist. eassumption.
-           rewrite max_env_max_value_eq. lia. }      
-        
-      rewrite (plus_comm _ a), plus_assoc. eapply plus_le_compat.
-      * rewrite (NPeano.Nat.mul_add_distr_r _ a). rewrite (plus_comm (_ * _) (_ * _)).
-        eapply plus_le_compat. lia. 
-        eapply mult_le_compat_l. eapply plus_le_compat_l. eapply mult_le_compat_l. eassumption.
-      * eassumption.
-    - (* proj *) intro; intros. intro; intros.
-      unfold inline_bound in *. 
-      eapply le_trans. eapply plus_le_compat_r. eassumption.
-      assert (Hleq : cost_exp_env G e1 (map_util.M.set x v1 rho1) <= cost_exp_env G (Eproj x t N y e1) rho1).
-      { unfold cost_exp_env. eapply Max.max_lub.
-        -- eapply le_trans; [| eapply Max.le_max_l ]. simpl. lia.
-        -- eapply le_trans. eapply max_env_set.
-           eapply Max.max_lub; [| lia ]. eapply le_trans; [| eapply Max.le_max_r ].
-           eapply le_trans; [| eapply max_env_get; eauto ]. simpl.
-           rewrite size_value_eq. eapply fold_left_max_in. eapply nthN_In. eassumption. }            
-      rewrite (plus_comm _ a), plus_assoc. eapply plus_le_compat.
-      * rewrite (NPeano.Nat.mul_add_distr_r _ a). rewrite (plus_comm (_ * _) (_ * _)).
-        eapply plus_le_compat. lia. 
-        eapply mult_le_compat_l. eapply plus_le_compat_l. eapply mult_le_compat_l. eassumption.
-      * eassumption.
-    - (* fun *) intro; intros. intro; intros.
-      unfold inline_bound in *.
-      eapply le_trans. eapply plus_le_compat_r. eassumption.
-      assert (Hleq : cost_exp_env G e1 (def_funs B1 B1 rho1 rho1) <= cost_exp_env G (Efun B1 e1) rho1). 
-      { unfold cost_exp_env. eapply Max.max_lub.
-        -- eapply le_trans; [| eapply Max.le_max_l ]. simpl. lia.
-        -- eapply le_trans. eapply max_env_def_funs. simpl. lia. }
-      rewrite (plus_comm _ a), plus_assoc. eapply plus_le_compat.
-      * rewrite (NPeano.Nat.mul_add_distr_r _ a). rewrite (plus_comm (_ * _) (_ * _)).
-        eapply plus_le_compat. lia. 
-        eapply mult_le_compat_l. eapply plus_le_compat_l. eassumption.
-      * eassumption.
-    - (* case hd *) intro; intros. intro; intros.
-      unfold inline_bound in *.
-      eapply le_trans. eapply plus_le_compat_r. eassumption.
-      assert (Hleq : cost_exp_env e1 rho1 <= cost_exp_env (Ecase x ((t, e1) :: B1)) rho1).
-      { unfold cost_exp_env. eapply Nat.max_le_compat_r.
-        simpl. lia. }
-      rewrite (plus_comm _ a), plus_assoc. eapply plus_le_compat.
-      * rewrite (NPeano.Nat.mul_add_distr_r _ a). rewrite (plus_comm (_ * _) (_ * _)).
-        eapply plus_le_compat. lia. 
-        eapply mult_le_compat_l. eapply plus_le_compat_l.
-        simpl. eassumption.
-      * eassumption.
-    - (* case tl *) intro; intros. intro; intros.
-      unfold inline_bound in *.
-      eapply le_trans. eassumption.
-      assert (Hleq : cost_exp_env (Ecase x B1) rho1 <= cost_exp_env (Ecase x ((t, e1) :: B1)) rho1).
-      { unfold cost_exp_env. eapply Nat.max_le_compat_r. simpl. lia. }
-      eapply plus_le_compat.
-      * eapply mult_le_compat_l. eapply plus_le_compat_l. eassumption.
-      * eassumption.
-    - (* app *) intro; intros. intro; intros.  
-      unfold inline_bound in *.
-      eapply le_trans. eapply plus_le_compat_r. eassumption.
-      assert (Hleq : cost_exp_env e1 rhoc1' <= cost_exp_env (Eapp x t xs) rho1).
-      { unfold cost_exp_env at 2. eapply le_trans; [| eapply Max.le_max_r ].
-        unfold cost_exp_env. eapply Nat.max_lub.
-
-  Fixpoint size_exp (e : exp) : nat :=
-    match e with
-    | Econstr x _ ys e => 1 + length ys + size_exp e
-    | Ecase x l =>
-      1  + (fix size_l l :=
-              match l with
-              | [] => 0
-              | (t, e) :: l => max (size_exp e) (size_l l)
-              end) l
-    | Eproj x _ _ y e => 1 + size_exp e
-    | Eletapp x f _ ys e => 1 + length ys + size_exp e
-    | Efun B e => max (size_fundefs B) (1 + size_exp e)
-    | Eapp x _ ys => 1 + length ys
-    | Eprim x _ ys e => length ys + size_exp e
-    | Ehalt x => 1
-    end
-  with size_fundefs (B : fundefs) : nat := 
-    match B with
-    | Fcons _ _ xs e B => max (size_exp e) (size_fundefs B)
-    | Fnil => 0
-    end.
-
-    
-  Fixpoint size_value' (G : nat) (v : val) {struct v} :=
-    match v with
-    | Vconstr _ vs => fold_left (fun m v => max m (size_value' G v)) vs 0
-    | Vfun rho B _ =>
-      let senv :=
-          (fix max_env m :=
-             match m with
-             | M.Leaf => 0
-             | M.Node l (Some v) r => max (size_value' G v) (max (max_env l) (max_env r))
-             | M.Node l None r => (max (max_env l) (max_env r))
-             end) rho in
-      G * max (size_fundefs B) senv
-    | Vint x => 0
-    end.
-
-  Fixpoint max_env {A} (f : A -> nat) (m : M.t A) :=
-    match m with
-    | M.Leaf => 0
-    | M.Node l (Some v) r => max (f v) (max (max_env f l) (max_env f r))
-    | M.Node l None r => (max (max_env f l) (max_env f r))
-    end.
-
-  Definition size_value (G : nat) (v : val) :=
-    match v with
-    | Vconstr _ vs => fold_left (fun m v => max m (size_value' G v)) vs 0
-    | Vfun rho B _ =>
-      G * max (size_fundefs B) (max_env (size_value' G) rho)
-    | Vint x => 0
-    end.
-
-  Lemma size_value_eq G v :
-    size_value G v = size_value' G v.
-  Proof.
-    destruct v.
-    - reflexivity.
-    - simpl. do 2 f_equal. induction t.
-      + reflexivity.
-      + simpl. destruct o; eauto.
-    - reflexivity.
-  Qed.
-  
-  Lemma max_env_f_eq {A} (f f' : A -> nat) rho :
-    (forall a, f a = f' a) ->
-    max_env f rho = max_env f' rho.
-  Proof.
-    induction rho; eauto; intros.
-    simpl. rewrite IHrho1, IHrho2; eauto. destruct o; eauto.
-  Qed.
-
-  Lemma max_env_max_value_eq G rho :
-    max_env (size_value' G) rho = max_env (size_value G) rho.
-  Proof.
-    erewrite max_env_f_eq. reflexivity.
-    intros. rewrite size_value_eq. reflexivity. 
-  Qed.
-  
-  Definition cost_exp_env G e rho := max (size_exp e) (max_env (size_value G) rho). 
-
-
-  Lemma fold_left_max_acc {A} l acc (f : A -> nat) :
-    fold_left (fun m v => max m (f v)) l acc = 
-    max (fold_left (fun m v => max m (f v)) l 0) acc. 
-  Proof.
-    revert acc; induction l; intros; simpl; eauto.
-    rewrite IHl. rewrite (IHl (f a)). lia.
-  Qed.
-
-
-  Lemma fold_left_max_in {A} l (x : A) acc f :
-    List.In x l ->
-    f x <= fold_left (fun m v => max m (f v)) l acc. 
-  Proof.
-    revert acc; induction l; intros acc Hin. now inv Hin.
-    simpl. inv Hin.
-    - simpl. rewrite fold_left_max_acc. lia.
-    - eapply le_trans. eapply IHl. eassumption. reflexivity.
-  Qed.
-
-
-  Lemma max_env_set {A} (f : A -> nat) rho x v :
-    max_env f (M.set x v rho) <= max (f v) (max_env f rho).
-  Proof.
-    revert rho. induction x; intros.
-    - destruct rho; simpl; eauto.
-      + rewrite IHx. simpl. reflexivity.
-      + destruct o; specialize (IHx rho2); lia.
-    - destruct rho; simpl; eauto.
-      + specialize (IHx M.Leaf). simpl in *. lia.
-      +  destruct o; specialize (IHx rho1); lia.
-    - simpl. destruct rho. simpl. lia.
-      simpl. destruct o; simpl; lia.
-  Qed.      
-
-  Lemma max_env_setlist {A} (f : A -> nat) rho rho' xs vs :
-    set_lists xs vs rho = Some rho' -> 
-    max_env f rho' <= max (fold_left (fun m v => max m (f v)) vs 0) (max_env f rho).
-  Proof.
-    revert rho rho' vs. induction xs; intros.
-    - destruct vs; inv H. lia.
-    - simpl in H. destruct vs. inv H.
-      destruct (set_lists xs vs rho) eqn:Heqs; inv H.
-      simpl. rewrite fold_left_max_acc. eapply le_trans.
-      eapply max_env_set. eapply Max.max_lub. lia.
-      eapply le_trans. eapply IHxs; eauto. lia. 
-  Qed.
-
-  Require Import identifiers.
-
-
-  Lemma size_fundefs_fun_in_fundefs B xs t e :
-    fun_in_fundefs B (xs, t, e) ->
-    size_exp e <= size_fundefs B.
-  Proof.
-    induction B; intros Hbin; inv Hbin.
-    - inv H. simpl. lia.
-    - eapply le_trans. eapply IHB. eassumption. simpl. lia.
-  Qed.
-    
-  Lemma max_env_def_funs G rho B B0 :
-    max_env (size_value G) (def_funs B0 B rho rho) <=
-    max (G * max (size_fundefs B0) (max_env (size_value G) rho)) (max_env (size_value G) rho).
-  Proof.
-    induction B; simpl; [| lia ].
-    
-    eapply le_trans. eapply max_env_set. eapply Nat.max_lub.
-    + simpl. rewrite max_env_max_value_eq. lia.
-    + lia.
-  Qed.
-
-  
-  Lemma max_env_get {A} (f : A -> nat) rho x v :
-    M.get x rho = Some v ->
-    f v <= max_env f rho. 
-  Proof.
-    revert rho. induction x; simpl; intros.
-    - destruct rho. congruence. eapply IHx in H.
-      eapply le_trans. eassumption. destruct o; simpl; lia.
-    - destruct rho. congruence. eapply IHx in H.
-      eapply le_trans. eassumption. destruct o; simpl; lia.
-    - destruct rho. congruence. destruct o; simpl in H; inv H.
-      simpl; lia.
-  Qed.
-
-    
-  Lemma max_env_getlist {A} (f : A -> nat) rho xs vs :
-    get_list xs rho = Some vs ->
-    fold_left (fun m v => max m (f v)) vs 0 <= max_env f rho. 
-  Proof.
-    revert vs rho. induction xs; intros.
-    + inv H. simpl. lia.
-    + simpl in H. destruct (rho ! a) eqn:Hgeta; try congruence.
-      destruct (get_list xs rho) eqn:Hgetl; try congruence.
-      inv H. simpl. rewrite fold_left_max_acc. eapply Max.max_lub.
-      * eapply IHxs. eassumption.
-      * eapply max_env_get. eassumption.
-  Qed.
-
-
-  
-  (* (possible) bound for inlining *)
-  Definition inline_bound (i G : nat) : relation (exp * env *  nat) := 
-    fun '(e1, rho1, c1) '(e2, rho2, c2) =>
-      c1 <= c2 * (1 + i * cost_exp_env G e1 rho1) + cost_exp_env G e1 rho1.
-
-  Context (cenv : ctor_env).
-  
-  Instance inline_bound_compat i G (Hi : i <= G) :
-    Post_properties cenv (inline_bound i G) (inline_bound i G) (inline_bound G G). 
-  Proof.
-    constructor.
-    11:{ intro; intros. unfold inline_bound in *.
-         destruct x as [[? ? ] ?]. destruct y as [[? ? ] ?]. eapply le_trans. eassumption.
-         eapply plus_le_compat_r. eapply mult_le_compat_l. eapply plus_le_compat_l.
-         eapply mult_le_compat_r. eassumption. }
-    
-    - (* constr *) intro; intros. intro; intros.
-      unfold inline_bound in *.
-      eapply le_trans. eapply plus_le_compat_r. eassumption.
-      assert (Hleq : cost_exp_env G e1 (map_util.M.set x (Vconstr t vs) rho1) <= cost_exp_env G (Econstr x t ys e1) rho1).
-      { unfold cost_exp_env. eapply Max.max_lub.
-        -- eapply le_trans; [| eapply Max.le_max_l ]. simpl. lia.
-        -- eapply le_trans. eapply max_env_set.
-           eapply Max.max_lub; [| lia ]. eapply le_trans.
-           simpl. eapply max_env_getlist. eassumption.
-           rewrite max_env_max_value_eq. lia. }      
-        
-      rewrite (plus_comm _ a), plus_assoc. eapply plus_le_compat.
-      * rewrite (NPeano.Nat.mul_add_distr_r _ a). rewrite (plus_comm (_ * _) (_ * _)).
-        eapply plus_le_compat. lia. 
-        eapply mult_le_compat_l. eapply plus_le_compat_l. eapply mult_le_compat_l. eassumption.
-      * eassumption.
-    - (* proj *) intro; intros. intro; intros.
-      unfold inline_bound in *. 
-      eapply le_trans. eapply plus_le_compat_r. eassumption.
-      assert (Hleq : cost_exp_env G e1 (map_util.M.set x v1 rho1) <= cost_exp_env G (Eproj x t N y e1) rho1).
-      { unfold cost_exp_env. eapply Max.max_lub.
-        -- eapply le_trans; [| eapply Max.le_max_l ]. simpl. lia.
-        -- eapply le_trans. eapply max_env_set.
-           eapply Max.max_lub; [| lia ]. eapply le_trans; [| eapply Max.le_max_r ].
-           eapply le_trans; [| eapply max_env_get; eauto ]. simpl.
-           rewrite size_value_eq. eapply fold_left_max_in. eapply nthN_In. eassumption. }            
-      rewrite (plus_comm _ a), plus_assoc. eapply plus_le_compat.
-      * rewrite (NPeano.Nat.mul_add_distr_r _ a). rewrite (plus_comm (_ * _) (_ * _)).
-        eapply plus_le_compat. lia. 
-        eapply mult_le_compat_l. eapply plus_le_compat_l. eapply mult_le_compat_l. eassumption.
-      * eassumption.
-    - (* fun *) intro; intros. intro; intros.
-      unfold inline_bound in *.
-      eapply le_trans. eapply plus_le_compat_r. eassumption.
-      assert (Hleq : cost_exp_env G e1 (def_funs B1 B1 rho1 rho1) <= cost_exp_env G (Efun B1 e1) rho1). 
-      { unfold cost_exp_env. eapply Max.max_lub.
-        -- eapply le_trans; [| eapply Max.le_max_l ]. simpl. lia.
-        -- eapply le_trans. eapply max_env_def_funs. simpl. lia. }
-      rewrite (plus_comm _ a), plus_assoc. eapply plus_le_compat.
-      * rewrite (NPeano.Nat.mul_add_distr_r _ a). rewrite (plus_comm (_ * _) (_ * _)).
-        eapply plus_le_compat. lia. 
-        eapply mult_le_compat_l. eapply plus_le_compat_l. eassumption.
-      * eassumption.
-    - (* case hd *) intro; intros. intro; intros.
-      unfold inline_bound in *.
-      eapply le_trans. eapply plus_le_compat_r. eassumption.
-      assert (Hleq : cost_exp_env e1 rho1 <= cost_exp_env (Ecase x ((t, e1) :: B1)) rho1).
-      { unfold cost_exp_env. eapply Nat.max_le_compat_r.
-        simpl. lia. }
-      rewrite (plus_comm _ a), plus_assoc. eapply plus_le_compat.
-      * rewrite (NPeano.Nat.mul_add_distr_r _ a). rewrite (plus_comm (_ * _) (_ * _)).
-        eapply plus_le_compat. lia. 
-        eapply mult_le_compat_l. eapply plus_le_compat_l.
-        simpl. eassumption.
-      * eassumption.
-    - (* case tl *) intro; intros. intro; intros.
-      unfold inline_bound in *.
-      eapply le_trans. eassumption.
-      assert (Hleq : cost_exp_env (Ecase x B1) rho1 <= cost_exp_env (Ecase x ((t, e1) :: B1)) rho1).
-      { unfold cost_exp_env. eapply Nat.max_le_compat_r. simpl. lia. }
-      eapply plus_le_compat.
-      * eapply mult_le_compat_l. eapply plus_le_compat_l. eassumption.
-      * eassumption.
-    - (* app *) intro; intros. intro; intros.  
-      unfold inline_bound in *.
-      eapply le_trans. eapply plus_le_compat_r. eassumption.
-      assert (Hleq : cost_exp_env e1 rhoc1' <= cost_exp_env (Eapp x t xs) rho1).
-      { unfold cost_exp_env at 2. eapply le_trans; [| eapply Max.le_max_r ].
-        unfold cost_exp_env. eapply Nat.max_lub.
-        - eapply le_trans; [| eapply max_env_get; eauto ]. simpl.
-          eapply le_trans. 
-          eapply size_fundefs_fun_in_fundefs. eapply find_def_correct. eassumption.
-          lia.
-        - eapply le_trans. eapply max_env_setlist. eassumption. eapply Nat.max_lub.
-          + eapply le_trans. eapply max_env_getlist. eassumption. lia.
-          + eapply le_trans; [| eapply max_env_get; eauto ]. simpl.
-            eapply le_trans. eapply max_env_def_funs. rewrite max_env_max_value_eq. lia. }
-      rewrite (plus_comm _ a), plus_assoc. eapply plus_le_compat.
-      * rewrite (NPeano.Nat.mul_add_distr_r _ a). rewrite (plus_comm (_ * _) (_ * _)).
-        eapply plus_le_compat. lia. 
-        eapply mult_le_compat_l. eapply plus_le_compat_l. eassumption.
-      * eassumption.
-    - (* letapp *) intro; intros. intro; intros.
-      unfold inline_bound in *. admit. 
-      (* eapply le_trans. eapply plus_le_compat_r. eassumption. *)
-      (* assert (Hleq : cost_exp_env e1 rhoc1' <= cost_exp_env (Eapp x t xs) rho1). *)
-      (* { unfold cost_exp_env at 2. eapply le_trans; [| eapply Max.le_max_r ]. *)
-      (*   unfold cost_exp_env. eapply Nat.max_lub. *)
-      (*   - eapply le_trans; [| eapply max_env_get; eauto ]. simpl. *)
-      (*     eapply le_trans.  *)
-      (*     eapply size_fundefs_fun_in_fundefs. eapply find_def_correct. eassumption. *)
-      (*     lia. *)
-      (*   - eapply le_trans. eapply max_env_setlist. eassumption. eapply Nat.max_lub. *)
-      (*     + eapply le_trans. eapply max_env_getlist. eassumption. lia. *)
-      (*     + eapply le_trans; [| eapply max_env_get; eauto ]. simpl. *)
-      (*       eapply le_trans. eapply max_env_def_funs. rewrite max_env_max_value_eq. lia. } *)
-      (* rewrite (plus_comm _ a), plus_assoc. eapply plus_le_compat. *)
-      (* * rewrite (NPeano.Nat.mul_add_distr_r _ a). rewrite (plus_comm (_ * _) (_ * _)). *)
-      (*   eapply plus_le_compat. lia.  *)
-      (*   eapply mult_le_compat_l. eapply plus_le_compat_l. eassumption. *)
-      (* * eassumption. *)      
-      (* admit. *)
-    - (* letapp OOT *) intro; intros. intro; intros.
-      unfold inline_bound in *.
-      assert (Hleq : cost_exp_env e_b1 rhoc1' <= cost_exp_env (Eletapp x f t xs e1) rho1).
-      { unfold cost_exp_env at 2. eapply le_trans; [| eapply Max.le_max_r ].
-        unfold cost_exp_env. eapply Nat.max_lub.
-        - eapply le_trans; [| eapply max_env_get; eauto ]. simpl.
-          eapply le_trans. 
-          eapply size_fundefs_fun_in_fundefs. eapply find_def_correct. eassumption.
-          lia.
-        - eapply le_trans. eapply max_env_setlist. eassumption. eapply Nat.max_lub.
-          + eapply le_trans. eapply max_env_getlist. eassumption. lia.
-          + eapply le_trans; [| eapply max_env_get; eauto ]. simpl.
-            eapply le_trans. eapply max_env_def_funs. rewrite max_env_max_value_eq. lia. }      
-
-      eapply le_trans. eapply plus_le_compat_r. eassumption.
-      rewrite (plus_comm _ a), plus_assoc. eapply plus_le_compat.
-      * rewrite (NPeano.Nat.mul_add_distr_r _ a). rewrite (plus_comm (_ * _) (_ * _)).
-        eapply plus_le_compat. lia. 
-        eapply mult_le_compat_l. eapply plus_le_compat_l. eassumption.
-      * eassumption.
-    - (* OOT *) intro; intros. intro; intros. unfold inline_bound. lia.
-    - (* base *) intro; intros. intro; intros. unfold inline_bound. lia.
-  Admitted.
-
-  Lemma size_exp_ge_1 e :
-    1 <= size_exp e.
-  Proof.
-    induction e using exp_ind'; simpl; try lia.
-  Qed.
-  
-  Lemma cost_exp_size_exp e :
-    cost e <= size_exp e.
-  Proof.
-    induction e using exp_ind'; simpl; try lia.
-    assert (Hge := size_exp_ge_1 e). lia. 
-  Qed.
-  
-  Lemma inline_bound_Hpost_zero e1 rho1 e2 rho2 :
-    post_zero e1 rho1 e2 rho2 inline_bound.
-  Proof.
-    intro; intros. unfold inline_bound. simpl.
-    eapply le_trans; [| eapply le_trans; [ eapply cost_exp_size_exp with (e := e1) |] ].
-    lia. unfold cost_exp_env. lia.
-  Qed.
-
-  Lemma inline_bound_post_Eapp_l v t l rho1 x rho2 :
-    post_Eapp_l inline_bound inline_bound v t l rho1 x rho2.
-  Proof.
-    intro; intros. unfold inline_bound in *.
-
-    Require Import inline_letapp.
-           (HEletapp : remove_steps_letapp cenv P1 P1 P1)
-           (Eletapp' : remove_steps_letapp' cenv P1 P1 P1)
-           (Eletapp_OOT : remove_steps_letapp_OOT cenv P1 P1)
-           (Eletapp_OOT' : remove_steps_letapp_OOT' cenv P1 P1).
-
-      
-      
-  Context (K : nat -> env -> exp -> nat) (* in essence, the number of inlined applications *)
-          (M : nat -> env -> exp -> nat). (* The total overhead of all L6 transformations, generally different for each program *)
-          
-  (* TODO: maybe remove step-index k if not needed in bounds *)
-
-  Definition upper_boundG (k : nat) : relation (exp * env *  nat) := 
-    fun '(e1, rho1, c1) '(e2, rho2, c2) => c2 <= (M k rho1 e1) * (c1 + 1).
-
-  Definition lower_boundG (k : nat) : relation (exp * env * nat) := 
-    fun '(e1, rho1, c1) '(e2, rho2, c2) => c1 <= (K k rho1 e1) * (c2 + 1).
-
-  (* + 1 is needed in the lower bound ecause sourvce might time out 
-   * in say M steps but that may be 0 steps in target *)
-
-  (* + 1 is not technically needed in the upper bound but it makes 
-    things easier *)
-
-  Definition boundG (k : nat) : relation (exp * env *  nat) :=
-    relation_conjunction (lower_boundG k) (upper_boundG k).
- 
-  Definition upper_boundL (local : nat) (k : nat) (rho : env) (e : exp) : relation nat := 
-    fun c1 c2 => c2 + local <= M k rho e * (c1 + 1).
-
-  Definition lower_boundL (local : nat) (k : nat) (rho : env) (e : exp) : relation nat := 
-    fun c1 c2 => c1 <= K k rho e * (c2 + 1 + local).
-
-  Definition boundL (local : nat) (k : nat) (rho : env) (e : exp) : relation nat :=
-    relation_conjunction (lower_boundL local k rho e) (upper_boundL local k rho e).
-  
-  (* bound properties *)
-  
-  Lemma boundL_0_implies_boundG k e1 e2 rho1 rho2 c1 c2 : 
-    boundL 0 k rho1 e1 c1 c2 -> boundG k (e1, rho1, c1) (e2, rho2, c2).
-  Proof.
-    unfold boundL, boundG, lower_boundL, lower_boundG, upper_boundL, upper_boundG. 
-    intros [H1 H2]. split; eauto.
-    eapply le_trans. eassumption. 
-    eapply Nat_as_OT.mul_le_mono_l. omega. 
-    rewrite Nat_as_DT.add_0_r in H2. 
-    eapply le_trans. eassumption. 
-    eapply Nat_as_OT.mul_le_mono_l. omega.       
-  Qed.
-(*
-  (* Divergence preservation *)
-  Lemma cc_approx_exp_divergence pr cenv ct l e1 rho1 e2 rho2 :  
-    (forall k, cc_approx_exp pr cenv ct k (boundL l) boundG (e1, rho1) (e2, rho2)) ->
-    diverge pr cenv rho1 e1 -> 
-    diverge pr cenv rho2 e2.
-  Proof.
-    intros Hexp H1 c2. assert (Hd := H1). specialize (H1 (K*(c2 + 1 + l))).
-    edestruct Hexp as [v2 [c2' [Hs2 [Hp Hval]]]]. reflexivity. eassumption.
-    destruct v2; try contradiction.
-    assert (Hleq : c2 <= c2').
-    { destruct Hp as [Hp1 Hp2]. unfold lower_boundL in Hp1.  
-      eapply Nat_as_DT.mul_le_mono_pos_l in Hp1; eauto. omega. }
-    eapply bstep_fuel_OOT_monotonic; eassumption. 
-  Qed.
-*)
-
 End Bounds.
 
   
